dev/aarch64_clean/src/arith_native_aarch64.h
@@ -150,19 +150,17 @@ void mld_polyz_unpack_19_asm(int32_t *r, const uint8_t *buf,
     defined(MLD_CONFIG_REDUCE_RAM) || defined(MLD_UNIT_TEST)
 #define mld_poly_pointwise_montgomery_asm \
   MLD_NAMESPACE(poly_pointwise_montgomery_asm)
-void mld_poly_pointwise_montgomery_asm(int32_t *r, const int32_t *a,
-                                       const int32_t *b)
+void mld_poly_pointwise_montgomery_asm(int32_t *a, const int32_t *b)
 /* This must be kept in sync with the HOL-Light specification
  * in proofs/hol_light/aarch64/proofs/mldsa_pointwise.ml */
 __contract__(
-  requires(memory_no_alias(r, sizeof(int32_t) * MLDSA_N))
   requires(memory_no_alias(a, sizeof(int32_t) * MLDSA_N))
   requires(memory_no_alias(b, sizeof(int32_t) * MLDSA_N))
   /* check-magic: off */
   requires(array_abs_bound(a, 0, MLDSA_N, 75423753))
   requires(array_abs_bound(b, 0, MLDSA_N, 75423753))
-  assigns(memory_slice(r, sizeof(int32_t) * MLDSA_N))
-  ensures(array_abs_bound(r, 0, MLDSA_N, 8380417))
+  assigns(memory_slice(a, sizeof(int32_t) * MLDSA_N))
+  ensures(array_abs_bound(a, 0, MLDSA_N, 8380417))
   /* check-magic: on */
 );
 #endif /* !MLD_CONFIG_NO_SIGN_API || !MLD_CONFIG_NO_VERIFY_API || \
