mldsa/src/poly.c
@@ -460,17 +460,15 @@ void mld_poly_invntt_tomont(mld_poly *a)
 
 #if !defined(MLD_CONFIG_NO_SIGN_API) || !defined(MLD_CONFIG_NO_VERIFY_API) || \
     defined(MLD_CONFIG_REDUCE_RAM) || defined(MLD_UNIT_TEST)
-MLD_STATIC_TESTABLE void mld_poly_pointwise_montgomery_c(mld_poly *c,
-                                                         const mld_poly *a,
+MLD_STATIC_TESTABLE void mld_poly_pointwise_montgomery_c(mld_poly *a,
                                                          const mld_poly *b)
 __contract__(
   requires(memory_no_alias(a, sizeof(mld_poly)))
   requires(memory_no_alias(b, sizeof(mld_poly)))
-  requires(memory_no_alias(c, sizeof(mld_poly)))
   requires(array_abs_bound(a->coeffs, 0, MLDSA_N, MLD_NTT_BOUND))
   requires(array_abs_bound(b->coeffs, 0, MLDSA_N, MLD_NTT_BOUND))
-  assigns(memory_slice(c, sizeof(mld_poly)))
-  ensures(array_abs_bound(c->coeffs, 0, MLDSA_N, MLDSA_Q))
+  assigns(memory_slice(a, sizeof(mld_poly)))
+  ensures(array_abs_bound(a->coeffs, 0, MLDSA_N, MLDSA_Q))
 )
 {
   unsigned int i;
@@ -480,31 +478,31 @@ __contract__(
   for (i = 0; i < MLDSA_N; ++i)
   __loop__(
     invariant(i <= MLDSA_N)
-    invariant(array_abs_bound(c->coeffs, 0, i, MLDSA_Q))
+    invariant(array_abs_bound(a->coeffs, 0, i, MLDSA_Q))
+    invariant(array_abs_bound(a->coeffs, i, MLDSA_N, MLD_NTT_BOUND))
     decreases(MLDSA_N - i)
   )
   {
-    c->coeffs[i] = mld_montgomery_reduce((int64_t)a->coeffs[i] * b->coeffs[i]);
+    a->coeffs[i] = mld_montgomery_reduce((int64_t)a->coeffs[i] * b->coeffs[i]);
   }
-  mld_assert_abs_bound(c->coeffs, MLDSA_N, MLDSA_Q);
+  mld_assert_abs_bound(a->coeffs, MLDSA_N, MLDSA_Q);
 }
 
 MLD_INTERNAL_API
-void mld_poly_pointwise_montgomery(mld_poly *c, const mld_poly *a,
-                                   const mld_poly *b)
+void mld_poly_pointwise_montgomery(mld_poly *a, const mld_poly *b)
 {
 #if defined(MLD_USE_NATIVE_POINTWISE_MONTGOMERY)
   int ret;
   mld_assert_abs_bound(a->coeffs, MLDSA_N, MLD_NTT_BOUND);
   mld_assert_abs_bound(b->coeffs, MLDSA_N, MLD_NTT_BOUND);
-  ret = mld_poly_pointwise_montgomery_native(c->coeffs, a->coeffs, b->coeffs);
+  ret = mld_poly_pointwise_montgomery_native(a->coeffs, b->coeffs);
   if (ret == MLD_NATIVE_FUNC_SUCCESS)
   {
-    mld_assert_abs_bound(c->coeffs, MLDSA_N, MLDSA_Q);
+    mld_assert_abs_bound(a->coeffs, MLDSA_N, MLDSA_Q);
     return;
   }
 #endif /* MLD_USE_NATIVE_POINTWISE_MONTGOMERY */
-  mld_poly_pointwise_montgomery_c(c, a, b);
+  mld_poly_pointwise_montgomery_c(a, b);
 }
 #endif /* !MLD_CONFIG_NO_SIGN_API || !MLD_CONFIG_NO_VERIFY_API || \
           MLD_CONFIG_REDUCE_RAM || MLD_UNIT_TEST */
