proofs/hol_light/aarch64/proofs/subroutine_signatures.ml
@@ -30,18 +30,16 @@ let subroutine_signatures = [
 );
 ("mldsa_pointwise",
   ([(*args*)
-     ("r", "int32_t[static 256]", (*is const?*)"false");
-     ("a", "int32_t[static 256]", (*is const?*)"true");
+     ("a", "int32_t[static 256]", (*is const?*)"false");
      ("b", "int32_t[static 256]", (*is const?*)"true");
    ],
    "void",
    [(* input buffers *)
     ("a", "256"(* num elems *), 4(* elem bytesize *));
     ("b", "256"(* num elems *), 4(* elem bytesize *));
-    ("r", "256"(* num elems *), 4(* elem bytesize *));
    ],
    [(* output buffers *)
-    ("r", "256"(* num elems *), 4(* elem bytesize *));
+    ("a", "256"(* num elems *), 4(* elem bytesize *));
    ],
    [(* temporary buffers *)
    ])
